Rewrite loop rules using unfoldings.

theories/lang/cpp/logic/stmt.v
@@ -382,13 +382,12 @@ Module Type Stmt.
         wp ρ (Sseq (Sdecl (d :: nil) :: Sif None e thn els :: nil)) Q
         |-- wp ρ (Sif (Some d) e thn els) Q.
 
-    (** * Loops *)
-    (* The loop rules are phrased using loop invariants. An alternative
-     * is to use their 1-step unfoldings and a greatest-fixpoint.
-     *
-     * Inconsistency: Certain infinite loops can be optimized away
-     * in C/C++. E.g. [while (1);] can be optimized to [;]. The loop
-     * rules do not support these.
+    (* The loops are phrased using 1-step unfoldings and invariant rules are
+       proved using Löb induction.
+
+       Certain infinite loops can be optimized away in C/C++.
+       E.g. <<while (1);>> can be optimized to <<;>>.
+       The loop rules do not support these optimizations.
      *)
 
     (* loop with invariant `I` *)
@@ -400,9 +399,29 @@ Module Type Stmt.
           | rt => Q rt
           end).
 
-    Axiom wp_while : forall ρ test body Q I,
-        I |-- wp ρ (Sif None test body Sbreak) (Kloop I Q) ->
+    (** * <<while>> *)
+
+    Definition while_unroll ρ test body :=
+      wp ρ (Sif None test body Sbreak).
+
+    Axiom wp_while_unroll : forall ρ test body Q,
+            while_unroll ρ test body (Kloop (|> wp ρ (Swhile None test body) Q) Q)
+        |-- wp ρ (Swhile None test body) Q.
+
+    Theorem wp_while_inv I : forall ρ test body Q,
+        I |-- while_unroll ρ test body (Kloop (|> I) Q) ->
         I |-- wp ρ (Swhile None test body) Q.
+    Proof.
+      intros.
+      iLöb as "IH".
+      iIntros "I".
+      iApply wp_while_unroll.
+      rewrite {2}H /while_unroll.
+      iRevert "I"; iApply wp_frame; first reflexivity.
+      iIntros (rt) "K"; destruct rt; simpl; eauto.
+      - iApply "IH"; eauto.
+      - iApply "IH"; eauto.
+    Qed.
 
     (**
        `while (T x = e) body` desugars to `{ T x = e; while (x) body }`
@@ -411,20 +430,47 @@ Module Type Stmt.
             wp ρ (Sseq (Sdecl (d :: nil) :: Swhile None test body :: nil)) Q
         |-- wp ρ (Swhile (Some d) test body) Q.
 
-    Axiom wp_for : forall ρ test incr body Q I,
-        let incr_I :=
-          match incr with
-          | None => I
-          | Some incr => wp_discard tu ρ incr (fun free => interp free I)
-          end
-        in
-        match test with
-        | None =>
-          I |-- wp ρ body (Kloop incr_I Q)
-        | Some test =>
-          I |-- wp ρ (Sif None test body Sbreak) (Kloop incr_I Q)
-        end ->
+    (** * <<for>> *)
+    Definition Kpost I Q :=
+      KP (fun rt =>
+            match rt with
+            | Normal | Continue => I
+            | _ => Q rt
+            end).
+
+    Definition for_unroll ρ test incr body (Q : Kpred) :=
+      let Kinc :=
+        Kpost (match incr with
+               | None => Q Normal
+               | Some incr => wp_discard tu ρ incr (fun free => interp free $ Q Normal)
+               end) Q
+      in
+      match test with
+      | None => wp ρ body
+      | Some test => wp ρ (Sif None test body Sbreak)
+      end Kinc.
+
+    Axiom wp_for_unroll : forall ρ test incr body Q,
+            for_unroll ρ test incr body (Kloop (|> wp ρ (Sfor None test incr body) Q) Q)
+        |-- wp ρ (Sfor None test incr body) Q.
+
+    Theorem wp_for_inv I : forall ρ test incr body Q,
+        I |-- for_unroll ρ test incr body (Kloop (|> I) Q) ->
         I |-- wp ρ (Sfor None test incr body) Q.
+    Proof.
+      intros.
+      iLöb as "IH".
+      iIntros "I".
+      iApply wp_for_unroll.
+      rewrite {2}H /for_unroll.
+      iRevert "I"; case_match; (iApply wp_frame; first reflexivity).
+      all: iIntros (rt); destruct rt; simpl; eauto.
+      all: case_match.
+      all: try (iApply wp_discard_frame; first reflexivity;
+                iIntros (?); iApply interp_frame;
+                iIntros "I !>"; iApply "IH"; eauto).
+      all: iIntros "I !>"; iApply "IH"; eauto.
+    Qed.
 
     (**
        `for (init; test; incr) body` desugars to `{ init; for (; test; incr) body }`
@@ -433,20 +479,33 @@ Module Type Stmt.
             wp ρ (Sseq (init :: Sfor None test incr b :: nil)) Q
         |-- wp ρ (Sfor (Some init) test incr b) Q.
 
-    (** ** `do` loops *)
+    (** * <<do>> *)
 
-    Definition Kdo (ρ : region) (e : Expr) (I : mpred) (Q : Kpred) : Kpred :=
-      KP (funI rt =>
-          match rt with
-          | Break => Q Normal
-          | Continue | Normal =>
-            Unfold WPE.wp_test (wp_test tu ρ e (fun c free => interp free $ if c then I else Q Normal))
-          | rt => Q rt
-          end).
+    Definition do_unroll ρ body test (Q : Kpred) :=
+      wp ρ body (Kpost (wp_test tu ρ test (fun c free => interp free $ if c then Q Continue else Q Break)) Q).
 
-    Axiom wp_do : forall ρ test body Q I,
-        I |-- wp ρ body (Kdo ρ test I Q) ->
+    Axiom wp_do_unroll : forall ρ body test Q,
+            do_unroll ρ body test (Kloop (|> wp ρ (Sdo body test) Q) Q)
+        |-- wp ρ (Sdo body test) Q.
+
+    Theorem wp_do_inv I : forall ρ body test Q,
+        I |-- do_unroll ρ body test (Kloop (|> I) Q) ->
         I |-- wp ρ (Sdo body test) Q.
+    Proof.
+      intros.
+      iLöb as "IH".
+      iIntros "I".
+      iApply wp_do_unroll.
+      rewrite {2}H /do_unroll.
+      iRevert "I"; iApply wp_frame; first reflexivity.
+      iIntros (rt) "K"; destruct rt; simpl; eauto.
+      { iRevert "K"; iApply wp_test_frame; iIntros (??).
+        iApply interp_frame; case_match; eauto.
+        iIntros "? !>"; iApply "IH"; eauto. }
+      { iRevert "K"; iApply wp_test_frame; iIntros (??).
+        iApply interp_frame; case_match; eauto.
+        iIntros "? !>"; iApply "IH"; eauto. }
+    Qed.
 
     (** * <<return>> *)
 
